x86/Reloctablesgenproof.v
@@ -35,16 +35,25 @@ Lemma transf_program_correct:
   forall rs, forward_simulation (RelocProgSemantics.semantics prog rs)
                                 (RelocProgSemantics1.semantics tprog rs).
 Proof.
+  intro rs.
+  eapply forward_simulation_step with (match_states := fun a b : Asm.state => a = b).
+  - simpl. unfold globalenv. simpl. unfold genv_senv. simpl.
+    unfold match_prog in TRANSF.
+    unfold transf_program in TRANSF.
+    monadInv TRANSF. unfold RelocProgSemantics.globalenv. intro id. simpl.
+    rewrite ! genv_senv_add_external_globals. simpl. auto.
+  - intros s1 IS. eexists; split; eauto.
+    unfold semantics. simpl. inv IS. simpl in *.
+    econstructor.
+
+
 Admitted.
 
 End PRESERVATION.
 
-Require Import RelocLinking.
+Require Import RelocLinking RelocLinking1.
 
-Instance reloctablesgen_linker : Linker RelocProgram.program.
-Admitted.
-
-Instance reloctablesgen_transflink : @TransfLink _ _ RelocLinking.Linker_reloc_prog reloctablesgen_linker match_prog.
+Instance reloctablesgen_transflink : @TransfLink _ _ RelocLinking.Linker_reloc_prog RelocLinking1.Linker_reloc_prog match_prog.
 Proof.
   red. simpl.
   unfold match_prog.
